modulo correctness proof

casestudy/modulo_ct_proof.ec
@@ -1,25 +1,11 @@
 require import AllCore IntDiv CoreMap List.
 from Jasmin require import JModel.
-
+require import Leakage_models.
 require Modulo_ct.
-
-op leak_div (a: W64.t) : int =
-  lzcnt (rev (w2bits a)).
-
-theory LeakageModelDiv.
-
-op leak_div_32 (a b: W32.t) : address list =
-  [ to_uint a ; to_uint b ].
-
-op leak_div_64 (a b: W64.t) : address list =
-  [ leak_div a ; to_uint b ].
-
-op leak_mem (a: address) : address = a.
-
-end LeakageModelDiv.
+import StdOrder.IntOrder Ring.IntID.
 
 clone import Modulo_ct.T with
-  theory LeakageModel <- LeakageModelDiv.
+  theory LeakageModel <-  LeakageModelTV.
 
 lemma leak_div_bound (w:W64.t) : 0 <= leak_div w <= 64.
 proof. smt (lzcnt_size size_mkseq size_rev). qed.
@@ -42,7 +28,7 @@ case: (64 = lzcnt (rev (mkseq ("_.[_]" x) 64))) => [<- /= /#| hdiff].
 case: (lzcnt (rev (mkseq ("_.[_]" x) 64)) = 0) => [-> /= [] // | ] /=.
 pose n := lzcnt _; pose X := bs2int _.
 move=> h0 h1; have /= /#: 2 ^ (64 - n) <= 2^63.
-apply StdOrder.IntOrder.ler_weexpn2l => //. smt (lzcnt_size size_mkseq size_rev).
+apply ler_weexpn2l => //. smt (lzcnt_size size_mkseq size_rev).
 qed.
 
 lemma shift_leak_div (b:W64.t) : 
@@ -52,15 +38,15 @@ proof.
   move=> hz; rewrite W64.to_uint_shl. smt (leak_div_bound).
   rewrite modz_small 2://. 
   split.
-  + apply StdOrder.IntOrder.mulr_ge0; 1: smt(W64.to_uint_cmp).
-    by apply StdOrder.IntOrder.expr_ge0.
+  + apply mulr_ge0; 1: smt(W64.to_uint_cmp).
+    by apply expr_ge0.
   move=> _; rewrite W64.to_uintE.
   have := lzcnt_bound (w2bits b).
   rewrite /leak_div size_w2bits (eq_sym 64) leak_div64 //= => -[] _. 
-  rewrite -(StdOrder.IntOrder.ltr_pmul2r (2 ^ lzcnt (rev (w2bits b)))).
-  + by apply StdOrder.IntOrder.expr_gt0.
-  rewrite -Ring.IntID.exprD_nneg //; 1,2: smt(leak_div_bound).
-  by rewrite Ring.IntID.subrK.
+  rewrite -(ltr_pmul2r (2 ^ lzcnt (rev (w2bits b)))).
+  + by apply expr_gt0.
+  rewrite -exprD_nneg //; 1,2: smt(leak_div_bound).
+  by rewrite subrK.
 qed.
 
 lemma shift_ZLCNT (b:W64.t) : 
@@ -80,9 +66,9 @@ proof.
   have := lzcnt_bound (w2bits b).
   rewrite size_w2bits (eq_sym 64) leak_div64 1:// /= -W64.to_uintE => -[h1 _].
   move: h1.
-  rewrite -(StdOrder.IntOrder.ler_pmul2r (2 ^ to_uint (W64.of_int (lzcnt (rev (w2bits b)))))).
-  + by rewrite StdOrder.IntOrder.expr_gt0.
-  rewrite -StdOrder.IntOrder.Domain.exprD_nneg; 1: smt(leak_div_bound leak_div64).
+  rewrite -(ler_pmul2r (2 ^ to_uint (W64.of_int (lzcnt (rev (w2bits b)))))).
+  + by rewrite expr_gt0.
+  rewrite -Domain.exprD_nneg; 1: smt(leak_div_bound leak_div64).
   + smt (W64.to_uint_cmp).
   rewrite W64.to_uint_small /=. smt (leak_div_bound ).
   have -> // : (63 - lzcnt (rev (w2bits b)) + lzcnt (rev (w2bits b))) = 63 by ring.
@@ -92,7 +78,7 @@ equiv l2 : M.mod_TV ~ M.mod_TV : ={M.leakages, b} /\ b{1} <> W64.zero ==> ={M.le
 proof.
   proc; inline *; wp; skip => /> &1 &2.
   move: (b{2}) (a{1}) (a{2}) => b a1 a2 {&1 &2} hb.
-  rewrite /leak_div_64; congr.
+  rewrite /leak_div_64 /leak_div_64_TV; congr.
   suff : forall a1,
    leak_div
      (if (if (LZCNT_64 a1).`5 then W64.one else if (LZCNT_64 b).`5 then W64.zero else W64.of_int 4660) = W64.zero then
@@ -124,7 +110,7 @@ proof.
   apply leak_div0.
   have heq: to_uint b * 2 ^ (leak_div b - 1) * 2 = to_uint b * 2 ^ leak_div b.
   + have {2}-> : 2 = 2 ^ 1 by done. 
-    rewrite mulzA -Ring.IntID.exprD_nneg //; 1: smt(leak_div_bound). 
+    rewrite mulzA -exprD_nneg //; 1: smt(leak_div_bound). 
   have h :  to_uint (b `<<<` leak_div b - 1) * 2 = to_uint (b `<<<` leak_div b).
   + have := shift_zlcnt b hb.
     rewrite shift_ZLCNT 1:// shift_leak_div 1:// => h.
@@ -147,7 +133,7 @@ lemma to_uint_lzcnt n : to_uint (of_int (lzcnt (rev (w2bits n))))%W64 = lzcnt (r
 proof.
   rewrite to_uint_small //.
   have := lzcnt_size (rev (w2bits n)).
-  smt.
+  rewrite /= size_rev size_w2bits /#.
 qed.
 
 lemma lzcnt0E w :
@@ -163,8 +149,8 @@ lemma lzcntn0E w :
 proof.
   rewrite /LZCNT_64 /ZF_of /= W64.to_uint_eq /= to_uint_lzcnt => w_not_big.
   have := lzcnt_bound (w2bits w).
-  rewrite size_w2bits -to_uintE.
-  smt.
+  have := lzcnt_size (rev (w2bits w)); rewrite size_rev size_w2bits -to_uintE.
+  have /# := ler_weexpn2l 2 _ (64 - lzcnt (rev (w2bits w))) 63=> //. 
 qed.
 
 hoare mod_TV_correct x y : M.mod_TV : arg = (x, y) /\ y <> W64.zero ==> res = x \umod y.
@@ -176,25 +162,30 @@ proof.
   move => /lzcntn0E[] x_not_big _.
   case: (LZCNT_64 y).`5.
   + move => /> /lzcnt0E y_big.
-    rewrite umodE /ulift2 /= modz_small //.
-    smt.
+    rewrite umodE /ulift2 /= modz_small ?to_uintK 2://; smt(W64.to_uint_cmp).
   move => /lzcntn0E[] y_not_big y_lzcnt_range.
   rewrite !W64.to_uint_eq /= /LEA_64 /addc /carry_add /b2i /=.
-  rewrite !/W64.(`<<`) W64.shlw_add 1, 2: #smt.
+  rewrite !/W64.(`<<`) W64.shlw_add 2://; 1: smt(W64.to_uint_cmp).
   rewrite /LZCNT_64 /truncateu8 /=.
-  rewrite to_uint_small. smt.
-  rewrite (modz_small _ 64). smt.
-  rewrite (modz_small _ 256). smt.
-  rewrite /=.
-  case: (18446744073709551616 <= to_uint (y `<<<` lzcnt (rev (w2bits y))) + to_uint x) => /= c;
-    rewrite umodE /ulift2 to_uintD_small.
-  + rewrite to_uint_shl 1: #smt.
-    admit.
-  + rewrite to_uint_shl 1: #smt.
-    rewrite (modz_small _ W64.modulus). admit.
-    by rewrite mulrC modzMDl.
-  + smt.
-  rewrite !/W64.(`<<`) to_uint_shl 1: #smt.
-  rewrite (modz_small _ W64.modulus). admit.
-  by rewrite mulrC modzMDl.
-admitted.
+  rewrite modz_dvd 1://.
+  rewrite to_uint_small; 1: smt (lzcnt_size size_rev size_w2bits).
+  rewrite (modz_small _ 64) /=; 1: smt (lzcnt_size size_rev size_w2bits). 
+  have heq: to_uint y * 2 ^ (leak_div y - 1) * 2 = to_uint y * 2 ^ leak_div y.
+  + have {2}-> : 2 = 2 ^ 1 by done. 
+    rewrite mulzA -exprD_nneg //; 1: smt(leak_div_bound).
+  have heq1 :  to_uint (y `<<<` leak_div y) = to_uint y * 2 ^ leak_div y.
+  + by rewrite -(shift_ZLCNT y y_nz) /LZCNT_64 /= to_uint_lzcnt.
+  have heq2 :  to_uint (y `<<<` leak_div y - 1) = to_uint y * 2 ^ (leak_div y - 1).
+  + have := shift_zlcnt y y_nz.
+    rewrite shift_ZLCNT 1:// => h. 
+    rewrite W64.to_uint_shl; 1: smt (leak_div_bound).
+    by rewrite modz_small //; move: heq h => /= /#.
+  have := shift_zlcnt y y_nz.
+  move: y_lzcnt_range x_not_big y_not_big; rewrite /LZCNT_64 /=  -/(leak_div y).
+  move => y_lzcnt_range x_not_big y_not_big.
+  rewrite W64.to_uint_small 1:/# => h1.
+  case: (18446744073709551616 <= to_uint (y `<<<` leak_div y) + to_uint x) => /= c;
+    rewrite umodE /ulift2 to_uintD_small 1:/#.
+  + by rewrite heq2 mulzC modzMDl.
+  by rewrite heq1 mulzC modzMDl.
+qed.
